more (unfinished)

thys/POPLmark/POPLmark_2B.thy
@@ -9,7 +9,58 @@ binder_datatype (FTVars: 'tv, FVars: 'v) trm = Var 'v
   | TApp "('tv, 'v) trm" "'tv typ"
 
 print_theorems
+(*TODO bindings FVars not used*)
+type_synonym "term" = "(var, var) trm"
 
-term Var
+inductive "value" where
+  "value (Abs x T t)"
+| "value (TAbs X T t)"
+
+inductive typing :: "\<Gamma>\<^sub>\<tau> \<Rightarrow> \<Gamma>\<^sub>\<tau> \<Rightarrow> term \<Rightarrow> type \<Rightarrow> bool" ("_ \<^bold>| _ \<^bold>\<turnstile> _ \<^bold>: _" [30,29,29,30] 30) where
+  TVar: "(x, T) \<in> set \<Gamma> \<Longrightarrow> \<Gamma> \<^bold>| \<Delta> \<^bold>\<turnstile> Var x \<^bold>: T"
+| TAbs: "\<Gamma> \<^bold>, x <: T1 \<^bold>| \<Delta> \<^bold>\<turnstile> t \<^bold>: T2 \<Longrightarrow> \<Gamma> \<^bold>| \<Delta> \<^bold>\<turnstile> Abs x T1 t \<^bold>: T1 \<rightarrow> T2"
+| TApp: "\<Gamma> \<^bold>| \<Delta> \<^bold>\<turnstile> t1 \<^bold>: T11 \<rightarrow> T12 \<Longrightarrow> \<Gamma> \<^bold>| \<Delta> \<^bold>\<turnstile> t2 \<^bold>: T11 \<Longrightarrow> \<Gamma> \<^bold>| \<Delta> \<^bold>\<turnstile> App t1 t2 \<^bold>: T12"
+| TTAbs: "\<Gamma> \<^bold>| \<Delta> \<^bold>, X <: T1 \<^bold>\<turnstile> t \<^bold>: T2 \<Longrightarrow> \<Gamma> \<^bold>| \<Delta> \<^bold>\<turnstile> TAbs X T1 t \<^bold>:  \<forall>X <: T1. T2"
+| TTApp: "\<Gamma> \<^bold>| \<Delta> \<^bold>\<turnstile> t1 \<^bold>: \<forall>X <: T11. T12 \<Longrightarrow> \<Delta> \<turnstile> T2 <: T11 \<Longrightarrow> \<Gamma> \<^bold>| \<Delta> \<^bold>\<turnstile> TApp t1 T2 \<^bold>: tvsubst_typ (TyVar(X := T2)) T12"
+| TSub: "\<Gamma> \<^bold>| \<Delta> \<^bold>\<turnstile> t \<^bold>: S \<Longrightarrow> \<Delta> \<turnstile> S <: T \<Longrightarrow> \<Gamma> \<^bold>| \<Delta> \<^bold>\<turnstile> t \<^bold>: T"
+
+lemma VVr_eq_TyVar[simp]: "tvVVr_tvsubst_typ a = TyVar a"
+  unfolding tvVVr_tvsubst_typ_def Var_def comp_def tv\<eta>_typ_tvsubst_typ_def TyVar_def
+  by (rule refl)
+
+lemma SSupp_typ_TyVar[simp]: "SSupp_typ TyVar = {}"
+  unfolding SSupp_typ_def by simp
+
+lemma SSupp_typ_fun_upd_le: "SSupp_typ (f(X := T)) \<subseteq> insert X (SSupp_typ f)"
+  unfolding SSupp_typ_def by auto
+
+lemma SSupp_typ_fun_upd_bound[simp]: "|SSupp_typ (f(X := T))| <o |UNIV :: var set| \<longleftrightarrow> |SSupp_typ f| <o |UNIV :: var set|"
+  apply safe
+   apply (metis SSupp_typ_fun_upd_le card_of_mono1 fun_upd_idem_iff fun_upd_upd infinite_UNIV insert_bound ordLeq_ordLess_trans)
+  apply (meson SSupp_typ_fun_upd_le card_of_mono1 infinite_UNIV insert_bound ordLeq_ordLess_trans)
+  done
+
+binder_inductive typing
+subgoal for R B \<sigma> \<Gamma> T1 T2
+    unfolding split_beta
+    by (elim disj_forward exE)
+      (auto simp add: isPerm_def supp_inv_bound map_context_def[symmetric] typ.vvsubst_permute trm.vvsubst_permute in_context_eqvt ty.equiv[folded map_context_def]
+        typ.permute_comp trm.permute_comp typ.FVars_permute trm.FVars_permute trm.permute_id wf_eqvt extend_eqvt lfset.set_map lfin_map_lfset induct_rulify_fallback
+        fun_eq_iff typ.tvsubst_permutes[THEN fun_cong, simplified] intro!: arg_cong[where f = "\<lambda>f. tvsubst_typ f _"]
+        | ((rule exI[of _ "\<sigma> _"] exI)+, (rule conjI)?, rule refl)
+        | ((drule spec2)+, (drule mp)?, assumption)
+        | ((rule exI[of _ "permute_typ \<sigma> _"])+, (rule conjI)?))+
+  subgoal premises prems for R B \<Gamma> \<Delta> t T
+
+    find_consts name: FVars
+    apply (tactic \<open>refreshability_tac true
+      [@{term "\<lambda>\<Gamma>. dom \<Gamma> \<union> FFVars_ctxt \<Gamma>"}, @{term "\<lambda>\<Delta>. dom \<Delta> \<union> FFVars_ctxt \<Delta>"}, @{term "\<lambda>t :: term. FVars_trm1 t \<union> FVars_trm2 t"}, @{term "FVars_typ :: type \<Rightarrow> var set"}]
+      [@{term "\<lambda>f. permute_trm f f :: term \<Rightarrow> term"}, @{term "permute_typ :: (var \<Rightarrow> var) \<Rightarrow> type \<Rightarrow> type"}, @{term "(\<lambda>f x. f x) :: (var \<Rightarrow> var) \<Rightarrow> var \<Rightarrow> var"}]
+      [NONE, SOME [NONE, SOME 2, NONE, NONE, SOME 0, NONE], NONE, NONE, NONE, NONE]
+      @{thm prems(3)} @{thm prems(2)} @{thms }
+      @{thms emp_bound insert_bound ID.set_bd trm.Un_bound trm.UN_bound trm.set_bd_UNIV typ.set_bd_UNIV infinite_UNIV}
+      @{thms typ_inject image_iff} @{thms typ.permute_cong_id context_map_cong_id map_idI}
+      @{thms } @{context}\<close>)
+  done
 
 end
